[WIP] UnifLogic: towards consume/produce...

theories/Base.v
@@ -229,6 +229,10 @@ Module Type BaseMixin (Import TY : Types).
       | exp_record R es    => term_record R (env.map (fun _ => seval_exp) es)
       end%exp.
 
+  Definition seval_exps {Γ Σ N} (δ : SStore Γ Σ) {Δ} :
+    NamedEnv (X := N) (Exp Γ) Δ -> NamedEnv (Term Σ) Δ
+      := env.map (fun b (e : Exp Γ (type b)) => peval (seval_exp δ e)).
+
   Lemma eval_exp_inst {Γ Σ τ} (ι : Valuation Σ) (δΓΣ : SStore Γ Σ) (e : Exp Γ τ) :
     eval e (inst δΓΣ ι) = inst (seval_exp δΓΣ e) ι.
   Proof.
